Charge!/src/Charge/ModularFunc/BaseType.v
@@ -16,7 +16,7 @@ Class BaseType (typ : Type) := {
   tyNat  : typ;
   tyBool : typ;
   tyString : typ;
-  tyPair : typ -> typ -> typ
+  tyProd : typ -> typ -> typ
 }.
 
 Section BaseTypeD.
@@ -26,7 +26,7 @@ Section BaseTypeD.
 	  btNat : typD tyNat = nat;
 	  btBool : typD tyBool = bool;
 	  btString : typD tyString = string;
-	  btPair : forall t1 t2, typD (tyPair t1 t2) = (typD t1 * typD t2)%type
+	  btProd : forall t1 t2, typD (tyProd t1 t2) = (typD t1 * typD t2)%type
 	}.
 	
 End BaseTypeD.
@@ -43,19 +43,68 @@ Section BaseTypeD'.
   Definition stringD (s : typD tyString) : string :=
     eq_rect _ id s _ btString.
 
-  Definition pairD (t1 t2 : typ) (p : typD (tyPair t1 t2)) : (typD t1 * typD t2)%type :=
-    eq_rect _ id p _ (btPair t1 t2).
+  Definition prodD (t1 t2 : typ) (p : typD (tyProd t1 t2)) : (typD t1 * typD t2)%type :=
+    eq_rect _ id p _ (btProd t1 t2).
     
-  Definition natD_sym (n : nat) : typD tyNat :=
+  Definition natR (n : nat) : typD tyNat :=
     eq_rect _ id n _ (eq_sym btNat).
 
-  Definition boolD_sym (b : bool) : typD tyBool :=
+  Definition boolR (b : bool) : typD tyBool :=
     eq_rect _ id b _ (eq_sym btBool).
 
-  Definition stringD_sym (s : string) : typD tyString :=
+  Definition stringR (s : string) : typD tyString :=
     eq_rect _ id s _ (eq_sym btString).
 
-  Definition pairD_sym (t1 t2 : typ) (p : (typD t1 * typD t2)%type) : typD (tyPair t1 t2) :=
-    eq_rect _ id p _ (eq_sym (btPair t1 t2)).
+  Definition prodR (t1 t2 : typ) (p : (typD t1 * typD t2)%type) : typD (tyProd t1 t2) :=
+    eq_rect _ id p _ (eq_sym (btProd t1 t2)).
     
+    
+  Lemma natDR n : natD (natR n) = n.
+  Proof.
+    unfold natD, natR, eq_rect_r, eq_rect, eq_sym, id.
+    destruct btNat; reflexivity.
+  Qed.
+
+  Lemma natRD n : natR (natD n) = n.
+  Proof.
+    unfold natD, natR, eq_rect_r, eq_rect, eq_sym, id.
+    destruct btNat; reflexivity.
+  Qed.
+
+  Lemma boolDR b : boolD (boolR b) = b.
+  Proof.
+    unfold boolD, boolR, eq_rect_r, eq_rect, eq_sym, id.
+    destruct btBool; reflexivity.
+  Qed.
+
+  Lemma boolRD b : boolR (boolD b) = b.
+  Proof.
+    unfold boolD, boolR, eq_rect_r, eq_rect, eq_sym, id.
+    destruct btBool; reflexivity.
+  Qed.
+  
+  Lemma stringDR s : stringD (stringR s) = s.
+  Proof.
+    unfold stringD, stringR, eq_rect_r, eq_rect, eq_sym, id.
+    destruct btString; reflexivity.
+  Qed.
+
+  Lemma stringRD s : stringR (stringD s) = s.
+  Proof.
+    unfold stringD, stringR, eq_rect_r, eq_rect, eq_sym, id.
+    destruct btString; reflexivity.
+  Qed.
+
+  Lemma prodDR t u p : prodD t u (prodR t u p) = p.
+  Proof.
+    unfold prodD, prodR, eq_rect_r, eq_rect, eq_sym, id.
+    destruct (btProd t u); reflexivity.
+  Qed.
+
+  Lemma prodRD t u p : prodR t u (prodD t u p) = p.
+  Proof.
+    unfold prodD, prodR, eq_rect_r, eq_rect, eq_sym, id.
+    destruct (btProd t u); reflexivity.
+  Qed.
+
 End BaseTypeD'.  
