Charge!/src/Charge/Tactics/Lists/Zip.v
@@ -1,3 +1,5 @@
+Require Import FunctionalExtensionality.
+
 Require Import MirrorCore.TypesI.
 Require Import MirrorCore.Lambda.AppN.
 Require Import MirrorCore.Lambda.Red.
@@ -10,6 +12,10 @@ Require Import Charge.ModularFunc.ListType.
 Require Import Charge.ModularFunc.BaseType.
 Require Import Charge.ModularFunc.SemiEqDecTyp.
 Require Import Charge.ModularFunc.Denotation.
+
+Require Import Charge.Tactics.Lists.ListTacs.
+Require Import Charge.Tactics.Base.DenotationTacs.
+Require Import Charge.Tactics.Base.MirrorCoreTacs.
 
 Require Import ExtLib.Core.RelDec.
 
@@ -37,12 +43,12 @@ Section Zip.
             match e2 with
               | App (App (Inj g) y) ys =>
                 match listS g with
-                  | Some (pCons _) => mkCons (tyPair t u) (mkPair t u x y) (zipExpr t u xs ys)
+                  | Some (pCons _) => mkCons (tyProd t u) (mkPair t u x y) (zipExpr t u xs ys)
                   | _ => mkZip t u e1 e2
                 end
               | Inj g =>
                 match listS g with
-                  | Some (pNil _) => mkNil (tyPair t u)
+                  | Some (pNil _) => mkNil (tyProd t u)
                   | _ => mkZip t u e1 e2
                 end
               | _ => mkZip t u e1 e2
@@ -51,23 +57,225 @@ Section Zip.
         end
       | Inj f =>
         match listS f with
-          | Some (pNil _) => mkNil (tyPair t u)
+          | Some (pNil _) => mkNil (tyProd t u)
           | _ => mkZip t u e1 e2
         end
       | _ => mkZip t u e1 e2
     end.
   
+  (* This function should have lst is it's third arguments, but for reasons that I cannot figure out at the moment
+     the function does not reduce with lst as the last argument. *)
+     
+  Fixpoint zipExprConst_left (t u : typ) (lst : list (typD u)) (e : expr typ func) : expr typ func :=
+    match lst with
+      | nil => mkNil (tyProd t u)
+      | y :: ys => 
+        match e with
+	      | App (App (Inj f) x) xs =>
+	        match listS f with
+	          | Some (pCons _) => mkCons (tyProd t u) (mkPair t u x (mkConst u y)) (zipExprConst_left t u ys xs)
+	          | _ => mkZip t u e (mkConst (tyList u) (listR lst))
+	        end
+	      | Inj f =>
+	        match listS f with
+	          | Some (pNil _) => mkNil (tyProd t u)
+	          | _ => mkZip t u e (mkConst (tyList u) (listR lst))
+	        end
+	      | _ => mkZip t u e (mkConst (tyList u) (listR lst))
+      end
+    end.
+(*  
+  Fixpoint zipExprConst_lefout (t u : typ) (e : expr typ func) (lst : list (typD u)) : expr typ func :=
+    match e with
+      | App (App (Inj f) x) xs =>
+        match listS f with
+          | Some (pCons _) =>
+            match lst with
+              | nil => mkNil (tyProd t u)
+              | y :: ys => mkCons (tyProd t u) (mkPair t u x (mkConst u y)) (zipExprConst_left t u xs ys)
+            end
+          | _ => mkZip t u e (mkConst (tyList u) (listR lst))
+        end
+      | Inj f =>
+        match listS f with
+          | Some (pNil _) => mkNil (tyProd t u)
+          | _ => mkZip t u e (mkConst (tyList u) (listR lst))
+        end
+      | _ => mkZip t u e (mkConst (tyList u) (listR lst))
+    end.
+  *)
+  Fixpoint zipExprConst_right (t u : typ) (lst : list (typD t)) (e : expr typ func) : expr typ func :=
+    match lst with
+      | nil => mkNil (tyProd t u)
+      | x :: xs => 
+        match e with
+	      | App (App (Inj f) y) ys =>
+	        match listS f with
+	          | Some (pCons _) => mkCons (tyProd t u) (mkPair t u (mkConst t x) y) (zipExprConst_right t u xs ys)
+	          | _ => mkZip t u (mkConst (tyList t) (listR lst)) e
+	        end
+	      | Inj f =>
+	        match listS f with
+	          | Some (pNil _) => mkNil (tyProd t u)
+	          | _ => mkZip t u (mkConst (tyList t) (listR lst)) e
+	        end
+	      | _ => mkZip t u (mkConst (tyList t) (listR lst)) e
+      end
+    end.
+  
+  Lemma zipExprConst_left_sound tus tvs (t u : typ) (xs : expr typ func) (ys : list (typD u))
+    (xsD : ExprI.exprT tus tvs (typD (tyList t)))
+    (Hxs : ExprDsimul.ExprDenote.exprD' tus tvs (tyList t) xs = Some xsD) :
+	ExprDsimul.ExprDenote.exprD' tus tvs (tyList (tyProd t u)) (zipExprConst_left t u ys xs) =
+	  Some (ExprDsimul.ExprDenote.exprT_App (ExprDsimul.ExprDenote.exprT_App (fun _ _ => zipD t u) xsD) (fun _ _ => listR ys)).
+  Proof.
+    generalize dependent xs. generalize dependent xsD.
+    induction ys; simpl; intros.
+    + rewrite listR_nil. 
+      unfold zipD, fun_to_typ2. 
+      do 2 rewrite exprT_App_wrap.
+      rewrite mkNil_sound.
+      rewriteD listD_nil. simpl.
+      unfold nilD, listR, eq_rect_r, eq_rect, eq_sym, id.
+      generalize (btProd t u). generalize (tyProd t u); intros.
+      generalize dependent (btList t0); intros.
+      generalize dependent (typD (tyList t0)); intros; subst.
+      generalize dependent (typD t0); intros; subst.
+      f_equal. do 2 (apply functional_extensionality; intro). destruct (listD (xsD x x0)); reflexivity.
+    + do 3 (destruct_exprs; try (apply mkZip_sound; [assumption | apply mkConst_sound])).
+      * reduce.
+        rewrite mkNil_sound.
+        unfold zipD, fun_to_typ2.
+        do 2 rewrite exprT_App_wrap.
+        rewrite listDR. rewrite listD_nil. simpl.
+        unfold nilD, listR, listD, eq_rect_r, eq_rect, eq_sym, id.
+        generalize (btProd t0 u). generalize (tyProd t0 u); intros.
+        generalize dependent (btList t); intros.
+        generalize dependent (typD (tyList t)).
+        generalize dependent (typD t).
+        intros; subst. reflexivity.
+      * do 2 (destruct_exprs; try (apply mkZip_sound; [assumption | apply mkConst_sound])).
+        reduce.
+        erewrite mkCons_sound; try eassumption; [| eapply mkPair_sound; [eassumption | apply mkConst_sound] | eapply IHys; eassumption].
+        unfold consD, zipD, pairD, fun_to_typ2.
+        do 8 rewrite exprT_App_wrap.
+        do 3 rewriteD listDR.
+        simpl. rewriteD listDR.
+        f_equal.
+        do 2 (apply functional_extensionality; intro).
+        f_equal.
+        unfold eq_rect_r, eq_rect, eq_sym, prodR, eq_rect, eq_sym. simpl.
+        generalize (btProd t0 u); generalize (e3 x x0, a); intros.
+        generalize dependent (typD (tyProd t0 u)); intros; subst. reflexivity.
+  Qed.
+
+  Lemma zipExprConst_right_sound tus tvs (t u : typ) (xs : list (typD t)) (ys : expr typ func) 
+    (ysD : ExprI.exprT tus tvs (typD (tyList u)))
+    (Hys : ExprDsimul.ExprDenote.exprD' tus tvs (tyList u) ys = Some ysD) :
+	ExprDsimul.ExprDenote.exprD' tus tvs (tyList (tyProd t u)) (zipExprConst_right t u xs ys) =
+	  Some (ExprDsimul.ExprDenote.exprT_App (ExprDsimul.ExprDenote.exprT_App (fun _ _ => zipD t u) (fun _ _ => listR xs)) ysD).
+  Proof.
+    generalize dependent ys. generalize dependent ysD.
+    induction xs; simpl; intros.
+    + rewrite listR_nil. 
+      unfold zipD, fun_to_typ2. 
+      do 2 rewrite exprT_App_wrap.
+      rewrite mkNil_sound.
+      rewriteD listD_nil. simpl.
+      unfold nilD, listR, eq_rect_r, eq_rect, eq_sym, id.
+      generalize (btProd t u). generalize (tyProd t u); intros.
+      generalize dependent (btList t0); intros.
+      generalize dependent (typD (tyList t0)); intros; subst.
+      generalize dependent (typD t0); intros; subst. reflexivity.
+    + destruct_exprs; try (reduce; apply mkZip_sound; [apply mkConst_sound | assumption]).
+      destruct_exprs; try (reduce; apply mkZip_sound; [apply mkConst_sound | reduce]).
+      destruct_exprs; try (apply mkZip_sound; [apply mkConst_sound | assumption]).
+      * reduce.
+        rewrite mkNil_sound.
+        unfold zipD, fun_to_typ2.
+        do 2 rewrite exprT_App_wrap.
+        rewrite listDR. simpl.
+        unfold nilD, listR, listD, eq_rect_r, eq_rect, eq_sym, id.
+        generalize (btProd t t0). generalize (tyProd t t0); intros.
+        generalize dependent (btList t1); intros.
+        generalize dependent (typD (tyList t1)).
+        generalize dependent (typD t1).
+        generalize dependent (btList t0).
+        generalize (tyList t0).
+        intros; subst.
+        generalize dependent (typD t2); intros; subst. reflexivity.
+      * do 4 (destruct_exprs; try (apply mkZip_sound; [apply mkConst_sound | assumption])).
+        reduce.
+        erewrite mkCons_sound; try eassumption; [| eapply mkPair_sound; [apply mkConst_sound | eassumption] | eapply IHxs; eassumption].
+        unfold consD, zipD, pairD, fun_to_typ2.
+        do 8 rewrite exprT_App_wrap.
+        do 3 rewriteD listDR.
+        simpl. rewriteD listDR.
+        f_equal.
+        do 2 (apply functional_extensionality; intro).
+        f_equal.
+        unfold eq_rect_r, eq_rect, eq_sym, prodR, eq_rect, eq_sym.
+        generalize (btProd t t0); generalize (a, e3 x x0); intros.
+        generalize dependent (typD (tyProd t t0)); intros; subst. reflexivity.
+  Qed.
+
+
   Lemma zipExprOk tus tvs (t u : typ) (xs ys : expr typ func) 
     (xsD : ExprI.exprT tus tvs (typD (tyList t))) (ysD : ExprI.exprT tus tvs (typD (tyList u)))
     (Hxs : ExprDsimul.ExprDenote.exprD' tus tvs (tyList t) xs = Some xsD)
     (Hys : ExprDsimul.ExprDenote.exprD' tus tvs (tyList u) ys = Some ysD) : 
-    ExprDsimul.ExprDenote.exprD' tus tvs (tyList (tyPair t u)) (zipExpr t u xs ys) =
+    ExprDsimul.ExprDenote.exprD' tus tvs (tyList (tyProd t u)) (zipExpr t u xs ys) =
       Some (ExprDsimul.ExprDenote.exprT_App (ExprDsimul.ExprDenote.exprT_App (fun _ _ => zipD t u) xsD) ysD).
   Proof.
     generalize dependent ys; generalize dependent xsD; generalize dependent ysD.
-    induction 
+    induction xs using expr_strong_ind; simpl; intros;
+      try (apply mkZip_sound; eassumption).
+    + do 2 (destruct_exprs; try (apply mkZip_sound; eassumption)).
+      reduce.
+      unfold zipD, fun_to_typ2.
+      do 2 rewrite exprT_App_wrap.
+      rewrite listD_nil. simpl.
+      rewrite mkNil_sound.
+      f_equal; do 2 (apply functional_extensionality; intro).
+      unfold nilD, listR, eq_rect_r, eq_rect, eq_sym, id.
+      generalize (btProd t0 u). generalize (tyProd t0 u); intros.
+      generalize dependent (btList t); intros.
+      generalize dependent (typD (tyList t)); intros; subst.
+      generalize dependent (typD t); intros; subst. reflexivity.
+    + do 7 (destruct_exprs; try (apply mkZip_sound; eassumption)).
+      * reduce.
+        unfold zipD, fun_to_typ2.
+        do 2 rewrite exprT_App_wrap.
+        rewrite listD_nil.
+        rewriteD listDR. simpl.
+        rewrite mkNil_sound.
+        unfold nilD, listR, eq_rect_r, eq_rect, eq_sym, id.
+        generalize (btProd t0 t1). generalize (tyProd t0 t1); intros.
+        generalize dependent (btList t); intros.
+        generalize dependent (typD (tyList t)); intros; subst.
+        generalize dependent (typD t); intros; subst. reflexivity.
+      * do 2 (destruct_exprs; try (apply mkZip_sound; eassumption)).
+        reduce.
+        unfold zipD, fun_to_typ2.
+        do 2 rewrite exprT_App_wrap.
+        erewrite mkCons_sound; [| eapply mkPair_sound; eassumption | eapply H; [repeat constructor | eassumption | eassumption]].
 
-  Definition zipTac (e : expr typ func) (args : list (expr typ func)) : expr typ func :=
+        do 6 (rewriteD exprT_App_wrap_sym).
+        unfold consD, zipD, pairD, fun_to_typ2.
+        do 6 rewriteD fun_to_typ_inv.
+        rewriteD listRD.
+        do 3 rewriteD listDR.
+        simpl.
+        rewriteD listDR.
+        f_equal.
+        do 2 (apply functional_extensionality; intro).
+        f_equal.
+        unfold eq_rect_r, eq_rect, eq_sym, prodR, eq_rect, eq_sym.
+        generalize (btProd t0 t1); generalize (e8 x x0, e4 x x0); intros.
+        generalize dependent (typD (tyProd t0 t1)); intros; subst. reflexivity.
+  Qed.
+    
+  Definition zipTac  (_ : list (option (expr typ func))) (e : expr typ func) (args : list (expr typ func)) : expr typ func :=
     match listS e with
       | Some (pZip t u) =>
         match args with
@@ -76,29 +284,58 @@ Section Zip.
               | Some (pConst v xs'), Some (pConst w ys') =>
                 match type_cast v (tyList t), type_cast w (tyList u) with
                   | Some pfxs, Some pfys =>
-                    mkConst (tyList (tyPair t u))
-                      (listD_inv _ (eq_rect _ list
-                        (combine (listD _ (eq_rect _ typD xs' _ pfxs))
-                           (listD _ (eq_rect _ typD ys' _ pfys))) _ (eq_sym (btPair t u))))
+                    mkConst (tyList (tyProd t u))
+                      (listR (eq_rect _ list
+                        (combine (listD (eq_rect _ typD xs' _ pfxs))
+                           (listD (eq_rect _ typD ys' _ pfys))) _ (eq_sym (btProd t u))))
                   | _, _ => apps e args
                 end 
               | Some (pConst v xs'), None => 
                 match type_cast v (tyList t) with
-                  | Some pf => zipExpr t u (list_const_to_expr t (listD _ (eq_rect _ typD xs' _ pf))) ys
+                  | Some pf => zipExprConst_right t u (listD (eq_rect _ typD xs' _ pf)) ys
                   | None => apps e args
                 end
               | None, Some (pConst v ys') => 
-                match type_cast v (tyList t) with
-                  | Some pf => zipExpr t u xs (list_const_to_expr t (listD _ (eq_rect _ typD ys' _ pf)))
+                match type_cast v (tyList u) with
+                  | Some pf => zipExprConst_left t u (listD (eq_rect _ typD ys' _ pf)) xs
                   | None => apps e args
                 end
-              | _, _ => apps e args
+              | _, _ => zipExpr t u xs ys
             end
           | _ => apps e args
         end
       | _ => apps e args
     end.
 
-Definition ZIP := SIMPLIFY (typ := typ) (fun _ _ _ _ => (beta_all (fun _ => zipTac))).
+  Lemma zipTacOk : partial_reducer_ok (zipTac nil).
+  Proof.
+    unfold partial_reducer_ok; intros.
+    eexists; split; [|reflexivity].
+    unfold zipTac.
+    do 6 (destruct_exprs; try assumption).
+    destruct_exprs; (try (reduce; apply zipExprOk; [reduce | eassumption])).
+    destruct_exprs. destruct e1; try congruence.
+    destruct_exprs; (try (reduce; apply zipExprOk; reduce)).
+    destruct_exprs; try assumption.
+    destruct_exprs; try assumption.
+	+ reduce.
+	  unfold zipD, fun_to_typ2.
+	  do 2 rewrite exprT_App_wrap. reflexivity.
+	+ destruct_exprs; try assumption.
+	  reduce.
+	  erewrite zipExprConst_right_sound; [|eassumption].
+	  unfold zipD, fun_to_typ2.
+	  do 4 rewrite exprT_App_wrap.
+	  rewriteD listDR. reflexivity.
+	+ do 2 (destruct_exprs; (try (reduce; apply zipExprOk; reduce; assumption))).
+      destruct_exprs; try assumption.
+      reduce.
+	  erewrite zipExprConst_left_sound; [|eassumption].
+	  unfold zipD, fun_to_typ2.
+	  do 3 rewrite exprT_App_wrap.
+	  rewrite listDR. reflexivity.
+  Qed.
+  
+Definition ZIP := SIMPLIFY (typ := typ) (fun _ _ _ _ => (beta_all zipTac)).
 
 End Zip.
