Charge!/src/Charge/Tactics/Base/BaseTacs.v
@@ -7,14 +7,44 @@ Require Import MirrorCore.TypesI.
 Require Import MirrorCore.ExprI.
 
 
+Ltac bf_const_type :=
+  match goal with
+    | H1 : baseS ?e = Some (pConst ?t ?c) |- _ =>
+      match goal with
+        | _ : ExprDsimul.ExprDenote.funcAs e t = Some _ |- _ => fail 1
+        | _ : ExprDsimul.ExprDenote.exprD' _ _ t e = Some _ |- _ => fail 1
+        | H2 : ExprDsimul.ExprDenote.funcAs e _ = Some _ |- _ =>
+  	  	  let H := fresh "H" in
+	        pose proof (bf_const_func_type_eq _ _ H1 H2) as H; repeat clear_eq; subst
+	    | H2 : ExprDsimul.ExprDenote.exprD' _ _ _ e = Some _ |- _ =>
+	      let H := fresh "H" in
+	        pose proof (bf_const_type_eq _ _ H1 H2) as H; repeat clear_eq; subst
+	  end
+  end.
+	  
+Ltac bf_const_expr :=
+  match goal with
+    | H1 : baseS ?e = Some (pConst ?t ?c) |- _ =>
+      match goal with
+        | _ : ExprDsimul.ExprDenote.exprD' _ _ t e =
+          Some (fun _ _ => c) |- _ => fail 1
+        | _ : ExprDsimul.ExprDenote.funcAs e t =
+   		  Some c |- _ => fail 1
+		| H2 : ExprDsimul.ExprDenote.funcAs e t = Some _ |- _ =>
+	 	  let H := fresh "H" in pose proof(bf_const_func_eq _ H1 H2); subst
+		| H2 : ExprDsimul.ExprDenote.exprD' _ _ t e = Some _ |- _ =>
+	  	  let H := fresh "H" in pose proof(bf_const_eq _ H1 H2); subst
+	 end
+   end.
+
 Ltac bf_forward_step :=
   match goal with 
     | H : Some _ = baseS _ |- _ =>  symmetry in H
-	| _ : baseS ?e = Some (pConst ?t ?c),
-	  _ : ExprDsimul.ExprDenote.exprD' _ _ ?t ?e = Some (fun _ _ => ?c) |- _ => fail 1
-	| H1 : baseS ?e = Some (pConst _ _), H2 : ExprDsimul.ExprDenote.exprD' _ _ _ ?e = Some _|- _ =>
-	  let H := fresh "H" in
-	     pose proof (bf_const_type_eq _ _ H1 H2) as H; r_inj H; repeat clear_eq; pose proof(bf_const_eq _ H1 H2); subst
+    | _ => 
+       first [
+        bf_const_type |
+        bf_const_expr
+      ]
   end.
     
 Ltac bf_rewrite_in_match :=
