Charge!/src/Charge/Tactics/Lists/ListTacs.v
@@ -1,5 +1,6 @@
 Require Import Charge.ModularFunc.ListFunc.
 Require Import Charge.ModularFunc.ListType.
+Require Import Charge.ModularFunc.BaseType.
 
 Require Import Charge.Tactics.Base.MirrorCoreTacs.
 
@@ -54,10 +55,10 @@ Ltac lf_nil_type :=
     | _ : listS ?e = Some (pNil ?t), _ : ExprDsimul.ExprDenote.exprD' ?tus ?tvs (tyList ?t) ?e = Some _ |- _ => fail 1
  	| H1 : listS ?e = Some (pNil _), H2 : ExprDsimul.ExprDenote.funcAs ?e _ = Some _ |- _ =>
 	  let H := fresh "H" in
-	     pose proof (lf_nil_func_type_eq _ _ H1 H2) as H; try list_inj H; repeat clear_eq; subst
+	     pose proof (lf_nil_func_type_eq _ _ H1 H2) as H; list_inj; repeat clear_eq; subst
 	| H1 : listS ?e = Some (pNil _), H2 : ExprDsimul.ExprDenote.exprD' _ _ _ ?e = Some _ |- _ =>
 	  let H := fresh "H" in
-	     pose proof (lf_nil_type_eq _ _ H1 H2) as H; try list_inj H; repeat clear_eq; subst
+	     pose proof (lf_nil_type_eq _ _ H1 H2) as H; list_inj; repeat clear_eq; subst
   end.
 
 Ltac lf_nil_expr :=
@@ -72,32 +73,66 @@ Ltac lf_nil_expr :=
 
 Ltac lf_cons_type :=
   match goal with
-    | _ : listS ?e = Some (pCons ?t), _ : ExprDsimul.ExprDenote.funcAs ?e (typ2 ?t (typ2 (tyList ?t) (tyList ?t))) = Some _ |- _ => fail 1
-    | _ : listS ?e = Some (pCons ?t), _ : ExprDsimul.ExprDenote.exprD' ?tus ?tvs (typ2 ?t (typ2 (tyList ?t) (tyList ?t))) ?e = Some _ |- _ => fail 1
- 	| H1 : listS ?e = Some (pCons _), H2 : ExprDsimul.ExprDenote.funcAs ?e _ = Some _ |- _ =>
-	  let H := fresh "H" in
-	     pose proof (lf_cons_func_type_eq _ _ H1 H2) as H; try (r_inj H); repeat clear_eq; subst
-	| H1 : listS ?e = Some (pCons _), H2 : ExprDsimul.ExprDenote.exprD' _ _ _ ?e = Some _ |- _ =>
-	  let H := fresh "H" in
-	     pose proof (lf_cons_type_eq _ _ H1 H2) as H; try (r_inj H); repeat clear_eq; subst
+    | H1 : listS ?e = Some (pCons ?t) |- _ =>
+      match goal with
+        | _ : ExprDsimul.ExprDenote.funcAs e (typ2 t (typ2 (tyList t) (tyList t))) = Some _ |- _ => fail 1
+        | _ : ExprDsimul.ExprDenote.exprD' _ _ (typ2 t (typ2 (tyList t) (tyList t))) e = Some _ |- _ => fail 1
+        | H2 : ExprDsimul.ExprDenote.funcAs e _ = Some _ |- _ =>
+  	  	  let H := fresh "H" in
+	        pose proof (lf_cons_func_type_eq _ _ H1 H2) as H; try (r_inj H); try list_inj; repeat clear_eq; subst
+	    | H2 : ExprDsimul.ExprDenote.exprD' _ _ _ e = Some _ |- _ =>
+	      let H := fresh "H" in
+	        pose proof (lf_cons_type_eq _ _ H1 H2) as H; try (r_inj H); try list_inj; repeat clear_eq; subst
+	  end
   end.
-
+	  
 Ltac lf_cons_expr :=
   match goal with
-    | _ : listS ?e = Some (pCons ?t),
-      _ : ExprDsimul.ExprDenote.exprD' _ _ (typ2 ?t (typ2 (tyList ?t) (tyList ?t))) ?e =
-     Some (fun _ _ => consD ?t) |- _ => fail 1
-    | _ : listS ?e = Some (pCons ?t),
-      _ : ExprDsimul.ExprDenote.funcAs ?e (typ2 ?t (typ2 (tyList ?t) (tyList ?t))) =
-     Some (consD ?t) |- _ => fail 1
-	| H1 : listS ?e = Some (pCons ?t),
-	  H2 : ExprDsimul.ExprDenote.funcAs ?e (typ2 ?t (typ2 (tyList ?t) (tyList ?t))) = Some _ |- _ =>
-	  let H := fresh "H" in pose proof(lf_cons_func_eq _ H1 H2); subst
-	| H1 : listS ?e = Some (pCons ?t),
-	  H2 : ExprDsimul.ExprDenote.exprD' _ _ (typ2 ?t (typ2 (tyList ?t) (tyList ?t))) ?e = Some _ |- _ =>
-	  let H := fresh "H" in pose proof(lf_cons_eq _ H1 H2); subst
-	| H : ExprDsimul.ExprDenote.exprD' _ _ (tyList ?t) (mkCons ?t _ _) = Some _ |- _ =>
+    | H1 : listS ?e = Some (pCons ?t) |- _ =>
+      match goal with
+        | _ : ExprDsimul.ExprDenote.exprD' _ _ (typ2 t (typ2 (tyList t) (tyList t))) _ =
+          Some (fun _ _ => consD t) |- _ => fail 1
+        | _ : ExprDsimul.ExprDenote.funcAs _ (typ2 t (typ2 (tyList t) (tyList t))) =
+   		  Some (consD t) |- _ => fail 1
+		| H2 : ExprDsimul.ExprDenote.funcAs e (typ2 t (typ2 (tyList t) (tyList t))) = Some _ |- _ =>
+	 	  let H := fresh "H" in pose proof(lf_cons_func_eq _ H1 H2); subst
+		| H2 : ExprDsimul.ExprDenote.exprD' _ _ (typ2 t (typ2 (tyList t) (tyList t))) e = Some _ |- _ =>
+	  	  let H := fresh "H" in pose proof(lf_cons_eq _ H1 H2); subst
+	 end
+    | H : ExprDsimul.ExprDenote.exprD' _ _ (tyList ?t) (mkCons ?t _ _) = Some _ |- _ =>
 	  pose proof (mkConsD _ _ _ H); clear H; (repeat destruct_match_oneres)
+  end.
+
+Ltac lf_zip_type :=
+  match goal with
+    | H1 : listS ?e = Some (pZip ?t ?u) |- _ =>
+      match goal with
+        | _ : ExprDsimul.ExprDenote.funcAs e (typ2 (tyList t) (typ2 (tyList u) (tyList (tyProd t u)))) = Some _ |- _ => fail 1
+        | _ : ExprDsimul.ExprDenote.exprD' _ _ (typ2 (tyList t) (typ2 (tyList u) (tyList (tyProd t u)))) e = Some _ |- _ => fail 1
+        | H2 : ExprDsimul.ExprDenote.funcAs e _ = Some _ |- _ =>
+  	  	  let H := fresh "H" in
+	        pose proof (lf_zip_func_type_eq _ _ H1 H2) as H; try (r_inj H); try list_inj; repeat clear_eq; subst
+	    | H2 : ExprDsimul.ExprDenote.exprD' _ _ _ e = Some _ |- _ =>
+	      let H := fresh "H" in
+	        pose proof (lf_zip_type_eq _ _ H1 H2) as H; try (r_inj H); try list_inj; repeat clear_eq; subst
+	  end
+  end.
+	  
+Ltac lf_zip_expr :=
+  match goal with
+    | H1 : listS ?e = Some (pZip ?t ?u) |- _ =>
+      match goal with
+        | _ : ExprDsimul.ExprDenote.exprD' _ _ (typ2 (tyList t) (typ2 (tyList u) (tyList (tyProd t u)))) _ =
+          Some (fun _ _ => zipD t u) |- _ => fail 1
+        | _ : ExprDsimul.ExprDenote.funcAs _ (typ2 (tyList t) (typ2 (tyList u) (tyList (tyProd t u)))) =
+   		  Some (zipD t u) |- _ => fail 1
+		| H2 : ExprDsimul.ExprDenote.funcAs e (typ2 (tyList t) (typ2 (tyList u) (tyList (tyProd t u)))) = Some _ |- _ =>
+	 	  let H := fresh "H" in pose proof(lf_zip_func_eq _ H1 H2); subst
+		| H2 : ExprDsimul.ExprDenote.exprD' _ _ (typ2 (tyList t) (typ2 (tyList u) (tyList (tyProd t u)))) e = Some _ |- _ =>
+	  	  let H := fresh "H" in pose proof(lf_zip_eq _ H1 H2); subst
+	 end
+    | H : ExprDsimul.ExprDenote.exprD' _ _ (tyList ?t) (mkCons ?t _ _) = Some _ |- _ =>
+	  pose proof (mkZipD _ _ _ H); clear H; (repeat destruct_match_oneres)
   end.
 
 Ltac lf_forward_step :=
@@ -108,11 +143,13 @@ Ltac lf_forward_step :=
         lf_nil_type |
         lf_fold_type |
         lf_map_type |
-        lf_nil_expr |
         lf_cons_type |
+        lf_zip_type |
+        lf_nil_expr |
         lf_cons_expr |
         lf_fold_expr |
-        lf_map_expr
+        lf_map_expr |
+        lf_zip_expr
       ]
   end.
  
